Working relation for initial state for cem and cbn

cbn_cem.v
@@ -2,7 +2,7 @@ Require cem cbn expr db relations.
 Require Import Minus.
 Require Import Unicode.Utf8 List NaryFunctions.
 Require Import expr_db util CpdtTactics.
-Require Import Basics.
+Require Import Basics EqNat.
 Require Import Compare_dec.
 
 Open Scope program_scope. 
@@ -20,7 +20,7 @@ Inductive lgexpr :=
 variables to debruijn indices and free variables to unmodified global variable
 *)
 Fixpoint etolg (e : expr.tm) (env : Map nat nat) :=  match e with
-  | expr.abs v b => etolg b ((v, 0):: map (fmap S) env)
+  | expr.abs v b => lam (etolg b ((v, 0):: map (fmap S) env))
   | expr.app m n => app (etolg m env) (etolg n env)
   | expr.var v => match lookup v env with
     | Some v' => lvar v'
@@ -149,56 +149,43 @@ Record configuration := conf {
 Definition eq_terms (t:expr.tm) (c:cem.configuration) : Prop := 
   Some (etolg t nil) = conftolg c 0.
 
-Fixpoint related_lists {a b} (la : list a) (lb : list b) (r : a → b → Prop) : Prop :=
-  match la, lb with
-  | x::xs, y::ys => r x y ∧ related_lists xs ys r
-  | nil, nil => True
-  | _, _ => False
-  end.
+Definition equal_heaps (h : cem.heap) (h' : cbn.heap) := related_lists (λ x y, match x,y with
+  | (l, cem.cl c e), (l', t) => l = l' ∧ eq_terms t (cem.conf h c)
+  end) h h'.
 
 Definition eq_confs (c: cem.configuration) (c':cbn.configuration) : Prop := 
+  cem.well_formed c ∧ cbn.well_formed c' ∧ 
   match c, c' with
-  | cem.conf h cl, cbn.st h' e' => eq_terms e' c ∧  related_lists h h' (λ x y, match x,y with
-    | (l, cem.cl c e), (l', t) => eq_terms t (cem.conf h c)
-    end)
+  | cem.conf h cl, cbn.st h' e' => eq_terms e' c ∧ equal_heaps h h'
   end.
 
-Lemma expr_closed_under_db: ∀ t xs, expr.fvs t ⊆ domain xs ↔ ∃ e, db t xs = Some e.
-intros t. induction t; intros; split; intros. simpl in H. destruct H. simpl.
-rewrite <- lookup_in_domain_iff in H.  destruct H. rewrite H. exists (db.var x).
-reflexivity. simpl in H. destruct H. remember (lookup n xs). symmetry in Heqo.
-destruct o. apply (ex_intro (λ n0, lookup n xs = Some n0) n0) in Heqo. apply
-lookup_in_domain in Heqo. simpl. split; auto. inversion H. simpl in H. rewrite
-app_subset_and in H. destruct H. apply IHt1 in H. apply IHt2 in H0. destruct H.
-destruct H0. simpl. rewrite H. rewrite H0. exists (db.app x x0). reflexivity.
-simpl in H. simpl. remember (db t1 xs). remember (db t2 xs). destruct o.
-destruct o0. symmetry in Heqo. symmetry in Heqo0. apply (ex_intro (λ x, db t1 xs
-= Some x) t) in Heqo. apply (ex_intro (λ x, db t2 xs = Some x) t0) in Heqo0.
-rewrite <- IHt1 in Heqo. rewrite <- IHt2 in Heqo0. rewrite app_subset_and; 
-split; auto. inversion H. inversion H0. inversion H. inversion H0. simpl in H.
-rewrite <- subset_remove_cons in H. rewrite <- domain_fmap with (f:=S) in H.
-specialize (IHt ((n,0)::map (fmap S) (xs))). simpl in IHt.
-apply IHt in H. simpl. destruct H. rewrite H. exists (db.lam x). reflexivity.
-destruct H. simpl in H. specialize (IHt ((n,0)::map (fmap S) xs)). remember (db
-t ((n,0)::map (fmap S) xs)). destruct o. inversion H. subst. symmetry in Heqo.
-destruct IHt. specialize (H1 (ex_intro (λ e, Some t0 = Some e) t0 eq_refl)).
-simpl. simpl in H1. rewrite domain_fmap in H1. rewrite <- subset_remove_cons.
-assumption. inversion H. Qed. 
+Lemma expr_closed_under_db: ∀ t xs, expr.fvs t ⊆ domain xs → {e | db t xs = Some e}.
+intros t. induction t; intros; simpl in H. destruct H. simpl.
+apply in_domain_lookup in H.  destruct H. rewrite e. exists (db.var x).
+reflexivity. 
 
-Lemma subset_map {A B} : ∀ xs ys (f:A→B), xs ⊆ ys → map f xs ⊆ map f ys. 
-intros xs. induction xs; intros. apply subset_nil. intros. simpl in H. simpl.
-split. destruct H. apply in_map. assumption. apply IHxs. destruct H. assumption.
-Qed. 
+rewrite app_subset_and in H. destruct H. apply IHt1 in H. apply IHt2 in H0.
+destruct H.  destruct H0. simpl. rewrite e. rewrite e0. exists (db.app x x0).
+reflexivity.   
 
-Definition homotopy {A B} (f g : A→B) := ∀ x, f x = g x.
-Notation "f ~ g" := (homotopy f g) (at level 60).  
+simpl in H. rewrite <- subset_remove_cons in H. rewrite <- domain_fmap with
+(f:=S) in H.  specialize (IHt ((n,0)::map (fmap S) (xs))). simpl in IHt.  apply
+IHt in H. simpl. destruct H. rewrite e. exists (db.lam x). reflexivity. Qed.
 
-Lemma snd_fmap {A} : (λ x:A*nat, pred (snd (fmap S x))) ~ (λ x:A*nat, snd x). 
-intros. unfold homotopy. intros. destruct x. reflexivity. Qed. 
+Lemma expr_db_closed_under : ∀ t xs e, db t xs = Some e → expr.fvs t ⊆ domain xs. 
+intros t. induction t; intros; simpl in H.
 
-Lemma map_homo {A B} : ∀ (f g:A→B), f ~ g → map f ~ map g. 
-unfold homotopy. intros. induction x. auto. simpl. rewrite H. rewrite IHx. auto.
-Qed. 
+destruct (lookup n xs) eqn:Heqo. apply lookup_domain in Heqo. simpl. split;
+auto. inversion H. 
+
+simpl. destruct (db t1 xs) eqn:Heqo. destruct (db t2 xs)
+eqn:Heqo0. apply IHt1 in Heqo. apply IHt2 in Heqo0. rewrite app_subset_and; 
+split; auto. inversion H. inversion H. 
+
+specialize (IHt ((n,0)::map (fmap S) xs)). destruct (db t ((n,0)::map (fmap S)
+xs)) eqn:Heqo. inversion H. subst. symmetry in Heqo. specialize (IHt t0
+eq_refl). simpl. simpl in IHt. rewrite domain_fmap in IHt. rewrite <-
+subset_remove_cons.  assumption.  inversion H. Qed.
 
 Lemma expr_db_closed : ∀ t e xs, db t xs = Some e → db.fvs e ⊆ codomain xs. 
 intros t. induction t; intros. inversion H. destruct (lookup n xs). inversion
@@ -214,12 +201,99 @@ rewrite map_map in Heqo. rewrite subset_remove_cons in Heqo. apply subset_map wi
 (f:=pred) in Heqo. rewrite map_map in Heqo. simpl. rewrite (map_homo _ _
 snd_fmap) in Heqo. assumption. inversion H1. Qed. 
 
+Fixpoint depth_env (xs : list nat) (y : nat) := match xs with 
+  | nil => y
+  | x::xs => if gt_dec (x+1) y then depth_env xs (x+1) else depth_env xs y
+  end.
 
-(*
-Lemma eq_initial_confs : ∀ t e, db t nil = Some e → eq_confs 
-  (cem.conf nil (cem.close e 0)) (cbn.st nil t).
-intros. split. unfold eq_terms. unfold conftolg. unfold etolg. induction t; simpl; intros. inversion H. destruct (db t1 nil).
-destruct (db t2 nil). inversion H. subst. split. unfold eq_terms. simpl.
+Lemma depth_env_y : ∀ xs y, y ≤ depth_env xs y. 
+intros xs. induction xs; intros. simpl. auto. simpl. destruct (gt_dec (a + 1)
+y). apply Gt.gt_S_le. specialize (IHxs (a + 1)). apply Gt.le_gt_trans
+with (p:=y) in IHxs; auto. apply IHxs. Qed. 
+
+Lemma depth_env_gt : ∀ xs y, forevery xs (λ x, depth_env xs y > x). 
+induction xs; intros. simpl. auto. simpl. destruct (gt_dec (a + 1) y). split.
+apply Gt.le_gt_trans with (m:=a+1). apply depth_env_y. rewrite Plus.plus_comm.
+simpl. auto. apply IHxs. split. apply Gt.le_gt_trans with (m:=y). apply
+depth_env_y. apply not_gt in n. rewrite Plus.plus_comm in n. simpl in n. apply
+Gt.le_S_gt. assumption. apply IHxs. Qed.  
+
+Lemma depth_env_map : ∀ xs y, S (depth_env xs y) = depth_env (map S xs) (S y). 
+induction xs. simpl. reflexivity. simpl. intros. destruct (gt_dec (a + 1) y).
+apply Gt.gt_n_S in g. destruct (gt_dec (S (a + 1)) (S y)). apply IHxs. apply n
+in g. inversion g. destruct (gt_dec (S (a+1)) (S y)). apply Gt.gt_S_n in g.
+apply n in g. inversion g. apply IHxs. Qed.   
+
+Lemma expr_db_eq : ∀ t e xs, db t xs = Some e → conftolg (cem.I e)
+  (depth_env (codomain xs) 0) = Some (etolg t xs).
+induction t; intros; subst. inversion H. destruct (lookup n xs) eqn:Heqo.
+inversion H1. subst. unfold conftolg. simpl. rewrite Heqo. apply lookup_codomain in Heqo.
+assert (depth_env (codomain xs) 0 > n0). rename xs into Xs. refine (forevery_in
+ _ _ _ Heqo (depth_env_gt _ _)). destruct (gt_dec (depth_env (codomain xs) 0)
+ n0). reflexivity. apply n1 in H0. inversion H0. inversion H1. inversion H.
+ destruct (db t1 xs) eqn:t1e. destruct (db t2 xs) eqn:t2e. specialize (IHt1 t
+ xs t1e). specialize (IHt2 t0 xs t2e). unfold conftolg. simpl. inversion H1.
+ subst. simpl. unfold conftolg in IHt1. simpl in IHt1. rewrite IHt1. unfold
+ conftolg in IHt2. simpl in IHt2. rewrite IHt2. simpl. reflexivity. inversion
+ t2e. inversion H1. inversion H1. simpl in H. destruct (db t ((n, 0) :: map
+ (fmap S) xs)) eqn:dbe. apply IHt in dbe. inversion H. subst. simpl in dbe.
+ simpl. rewrite depth_env_map. unfold codomain. unfold codomain in dbe. rewrite
+ map_map. rewrite map_map in dbe. rewrite map_homo with (g:=(λ x : nat * nat,
+ snd (fmap S x))). rewrite dbe. simpl. reflexivity. unfold homotopy. intros.
+ destruct x. simpl. reflexivity. inversion H. Qed.  
+
+Lemma expr_db_eq_confs : ∀ t e, db t nil = Some e → eq_confs (cem.I e) (cbn.I t).
+intros. split; split. simpl. apply expr_db_closed in H. apply subset_nil2 in H.
+rewrite H. simpl. auto. simpl. unfold cem.well_formed_heap. simpl. split. auto.
+apply unil. split. simpl. apply expr_db_closed_under in H. assumption. split.
+apply unil. simpl. auto. apply expr_db_eq in H. simpl. unfold eq_terms. rewrite
+<- H. simpl. split. reflexivity. apply rel_nil. Qed.  
+
+Lemma equal_heaps_domains : ∀ h h', equal_heaps h h' → domain h = domain h'. 
+intros. induction H. reflexivity. destruct x. destruct c. destruct y. destruct
+H. subst. simpl. f_equal. assumption. Qed.
+
+Lemma lu_inf' {A} : ∀ h l (c:A), lookup l h = Some c → 
+  ∃ Φ Ψ, h = Φ ++ (l, c) :: Ψ.
+induction h. intros. inversion H. intros. unfold lookup in H. simpl in H.
+destruct (EqNat.beq_nat l (fst a)) eqn:bne. destruct a. inversion H. subst.
+simpl in bne. apply beq_nat_true in bne. subst. exists nil, h.  simpl.
+reflexivity. apply beq_nat_false in bne. apply IHh in H. destruct H. destruct H.
+exists (a::x), x0. simpl. subst. reflexivity. Qed. 
+
+Lemma clu_inf' : ∀ x h e l c, cem.clu x e h = Some (l, c) → 
+  ∃ Φ Ψ e', h = Φ ++ (l, cem.cl c e') :: Ψ.
+induction x; intros. unfold cem.clu in H. destruct (lookup e h) eqn:lue.
+destruct c0. inversion H. subst. apply lu_inf' in lue. destruct lue. destruct
+H0. subst. exists x, x0, n. reflexivity. inversion H. assert (h':=H). apply
+clu_some_lu in h'. destruct h'. unfold cem.clu in H. rewrite H0 in H. destruct
+x0. apply IHx in H. destruct H. destruct H. destruct H. subst. exists x0, x1,
+x2.  reflexivity. Qed. 
+
+Lemma eq_confs_step1 : ∀ ce cb cb', eq_confs ce cb → cbn.step cb cb' → ∃ ce',
+  cem.step ce ce' ∧ eq_confs ce' cb'. 
+intros. generalize dependent ce. induction H0; intros; subst. destruct H.
+destruct H1. destruct ce. destruct H2. unfold eq_terms in H2. simpl in H2.
+destruct st_clos0. destruct clos_tm. simpl in H2. destruct (cem.clu (n - 0)
+clos_env st_heap0) eqn:clue. destruct p. unfold fmap_option in H2. unfold
+compose in H2. simpl in H2. inversion H2. subst. assert (infe:=clue). apply
+clu_inf' in infe. destruct infe. destruct H4. destruct H4. subst. specialize
+(IHstep (cem.conf (x ++ (n0, cem.cl c x1) :: x0) c)). exists
+(cem.conf (x ++ (n0, cem.cl c x1) :: x0) c). split. apply cem.Id. .   
+inversion H5. subst. exists (cem.conf st_heap0 (cem.close (db.var n) clos_env)).
+split. clos_env
+
+Lemma eq_initial_confs : ∀ e : {e | expr.closed e}, eq_confs 
+  (cem.I (proj1_sig (expr_closed_db e))) (cbn.I (proj1_sig e)).
+intros. destruct (expr_closed_db e) eqn:Heqe. generalize dependent x. simpl.
+induction e. generalize dependent p. induction x; intros; simpl; split; auto.
+unfold eq_terms. inversion p. assert (p':=p). apply app_eq_nil in p'. destruct
+p'. specialize (IHx1 H). specialize (IHx2 H0). unfold eq_terms. unfold
+expr_closed_db in Heqe.  unfold closed_expr_db in Heqe. simpl in Heqe. 
+destruct c'. specialize (IHx0_1 H). 
+unfold conftolg. unfold etolg. induction t; simpl; intros. inversion H. destruct
+(db t1 nil).  destruct (db t2 nil). inversion H. subst. split. unfold eq_terms.
+simpl.
 specialize (IHt1 t eq_refl). simpl in IHt1. unfold eq_terms in IHt1. subst; simpl. simpl in IHt1.
 simpl in IHt2. destruct (2simpl. unfold eq_confs. split. induction t. inversion H. inversion H. simpl. auto. 
 
